aneris/aneris_lang/adequacy_trace.v
@@ -1,61 +1,234 @@
-From aneris.aneris_lang Require Import aneris_lang proofmode adequacy_no_model.
+From trillium.prelude Require Import classical_instances.
+From trillium.program_logic Require Import language.
+From trillium Require Import finitary.
+From aneris.aneris_lang Require Import adequacy aneris_lang proofmode adequacy_no_model.
+From iris.base_logic.lib Require Import invariants.
 
-Definition heap_invariance `{anerisPreG Σ unit_model} (N : namespace) (I : list val → Prop) ip e σ :
+Definition aneris_invariance `{anerisPreG Σ unit_model} (N : namespace) (I : list val → Prop) 
+  ip e σ A IPs lbls obs_send_sas obs_rec_sas : 
+  state_heaps σ = {[ip:=∅]} →
+  state_sockets σ = {[ip:=∅]} →
+  state_ms σ = ∅ →
+  state_trace σ = [] →
+  ip ∉ IPs →
+  obs_send_sas ⊆ A →
+  obs_rec_sas ⊆ A →
   I (state_trace σ) →
-  (∀ `(anerisG Σ), ⊢ trace_inv N I -∗ trace_is (state_trace σ) -∗ WP e @[ip] ⊤ {{ _, True }}) →
+  (∀ `(anerisG Σ), ⊢ 
+    {{{ trace_inv N I ∗
+        trace_is (state_trace σ) ∗
+        unallocated A ∗
+        ([∗ set] a ∈ A, a ⤳[bool_decide (a ∈ obs_send_sas), bool_decide (a ∈ obs_rec_sas)] (∅, ∅)) ∗
+        ([∗ set] ip ∈ IPs, free_ip ip) ∗
+        ([∗ set] lbl ∈ lbls, alloc_evs lbl []) ∗
+        ([∗ set] sa ∈ obs_send_sas, sendon_evs sa []) ∗
+        ([∗ set] sa ∈ obs_rec_sas, receiveon_evs sa []) ∗
+        observed_send obs_send_sas ∗
+        observed_receive obs_rec_sas }}} 
+    e @[ip]
+    {{{ v, RET v; True }}}) →
   ∀ σ' t,
-    step ([(mkExpr ip e)], σ) (t, σ') →
+    rtc step ([(mkExpr ip e)], σ) (t, σ') →
     I (state_trace σ').
 Proof.
-  (* intros HI Hwp σ' t.
-  eapply (wp_invariance Σ _ s _ _ _ _ (I (trace σ'))). iIntros (Hinv κs) "".
-  iMod (gen_heap_init σ.(heap)) as (?) "Hh".
-  iMod (proph_map_init κs σ.(used_proph_id)) as (?) "Hp".
-  iMod (trace_auth_init σ.(trace)) as (?) "(Hta & Ht & Hth)".
-  iDestruct (inv_alloc N _ (∃ t, trace_half_frag t ∗ ⌜I t⌝) with "[Hth]") as ">#HI".
-  { iNext. eauto. }
-  iModIntro. iExists
-    (λ σ κs _, (gen_heap_ctx σ.(heap) ∗ trace_auth σ.(trace) ∗ proph_map_ctx κs σ.(used_proph_id))%I),
-    (λ _, True%I).
-  iFrame. iSplitL.
-  { iDestruct (Hwp (HeapG _ _ _ _ _)) as "Hwp". iApply ("Hwp" with "HI Ht"). }
-  iIntros "(_ & Hta & _)". iExists _.
-  iInv "HI" as ">Ht'" "_". iDestruct "Ht'" as (t') "(Ht' & %)".
-  iDestruct (trace_auth_half_frag_agree with "Hta Ht'") as %->. iModIntro. eauto.
-Qed. *)
-Admitted.
+  intros Hheaps Hsock Hms Htrace Hip_nin Hobs_send Hobs_rec HI Hwp σ' t Hsteps.
+  assert (@continued_simulation aneris_lang (aneris_to_trace_model unit_model)
+            (λ ex _, ∀ conf, trace_ends_in ex conf → I (state_trace conf.2))
+            (trace_singleton ([(mkExpr ip e)], σ))
+            (trace_singleton ())) as Hsim.
+  {
+    eapply (simulation_adequacy1 Σ (aneris_to_trace_model unit_model) 
+              NotStuck IPs lbls A obs_send_sas obs_rec_sas); try done.
+    - intros ?.
+      intros.
+      eapply finite_smaller_card_nat.
+      eapply (in_list_finite [((),())]).
+      intros state_label _.
+      destruct state_label as [u1 u2].
+      destruct u1, u2.
+      set_solver.
+      Unshelve.
+      intros.
+      apply make_proof_irrel.
+    - iIntros.
+      iModIntro.
+      iExists (λ v, (∃ w : val, ⌜v = {| val_n := ip; val_e := w |}⌝ ∗ True)%I).
+      iIntros "Hunalloc Hobs Hfree_ip His_node Hlbs Hsend_evs Hrec_evs 
+        Hobs_send Hobs_rec ? Hfrag_trace Htrace_is".
+      iMod (inv_alloc N _ (∃ t, trace_half_frag t ∗ ⌜I t⌝)%I with "[Hfrag_trace]") as "#Hinv".
+      {
+        iNext.
+        iExists [].
+        iFrame.
+        iPureIntro.
+        by rewrite -Htrace.
+      }
+      iModIntro.
+      iSplitL.
+      + unfold aneris_wp_def in Hwp.
+        iAssert (WP e @[ip] {{ _, True}}%I) with "[Hunalloc Hobs Hfree_ip 
+          Hlbs Hsend_evs Hrec_evs Hobs_send Hobs_rec Htrace_is]" as "Hwp".
+        {
+          iApply (Hwp anerisG0 with "[$Hinv Htrace_is $Hunalloc Hobs $Hfree_ip 
+            $Hlbs $Hsend_evs $Hrec_evs $Hobs_send $Hobs_rec][]"); try done.
+          rewrite Htrace.
+          iFrame.
+          unfold message_history_singleton.
+          simpl.
+          iApply (big_sepS_wand with "[$Hobs][]").
+          iApply big_sepS_intro.
+          iModIntro.
+          iIntros.
+          by iFrame.
+        }
+        rewrite !aneris_wp_unfold /aneris_wp_def.
+        iApply ("Hwp" with "[$His_node]").
+      + iIntros (?????????) "Hinterp ?".
+        simpl.
+        iInv "Hinv" as ">Hinv_res" "_".
+        iDestruct "Hinterp" as "(?&?&?&?&?& Hauth_trace)".
+        iApply fupd_mask_intro; first set_solver.
+        iIntros.
+        unfold trace_auth.
+        iDestruct "Hinv_res" as (t') "(Hinv_res1 & %Hinv_res2)".
+        iDestruct (trace_auth_half_frag_agree with "Hauth_trace Hinv_res1 ") as %<-.
+        iPureIntro.
+        intros.
+        apply last_eq_trace_ends_in in H6.
+        by rewrite H6 in Hinv_res2.
+  }
+  eapply (@trace_steps_rtc_bin _ unit) in Hsteps; last done.
+  destruct Hsteps as [ex (Htrace_steps & Htrace_start & Htrace_end)].
+  assert (∃ ex', trace_steps language.locale_step ex' ∧ 
+                 trace_starts_in ex' ([{| expr_n := ip; expr_e := e |}], σ) ∧
+                 trace_ends_in ex' (t, σ')) 
+                 as [ex' (Htrace_steps' & Htrace_start' & Htrace_end')].
+  {
+    clear Hwp Hsim Hheaps Hsock Hms Htrace HI.
+    generalize dependent t.
+    generalize dependent σ.
+    generalize dependent σ'.
+    induction Htrace_steps.
+    - intros.
+      exists {tr[ x ]}.
+      by split; first apply trace_steps_singleton.
+    - intros.
+      apply trace_extend_starts_in_inv in Htrace_start.
+      destruct x.
+      eapply IHHtrace_steps in Htrace_start; last apply H0.
+      destruct Htrace_start as 
+        [ex' (Htrace_steps' & Htrace_start' & Htrace_end')].
+      inversion H1.
+      + exists (ex' :tr[ (Some $ locale_of t1 e1) ]: y).
+        split.
+        * apply (trace_steps_step _ _ (l, s)); try done.
+          simplify_eq.
+          eapply locale_step_atomic; done.
+        * split; last done. 
+          by apply trace_extend_starts_in.
+      + exists (ex' :tr[ None ]: y).
+        split.
+        * apply (trace_steps_step _ _ (l, s)); try done.
+          simplify_eq.
+          eapply locale_step_state; done.
+        * split; last done. 
+          by apply trace_extend_starts_in.
+  }
+  assert (∃ atr, trace_starts_in atr () ∧ 
+                 continued_simulation 
+                 (λ (ex : execution_trace aneris_lang) 
+                    (_ : auxiliary_trace (aneris_to_trace_model unit_model)), 
+                     ∀ conf : cfg aneris_lang, trace_ends_in ex conf → 
+                                               I (state_trace conf.2)) 
+                  ex' atr) as [atr (_ & Hsim_ex')].
+  {
+    eapply (@simulation_does_continue 
+                        aneris_lang 
+                        (aneris_to_trace_model unit_model)); try done.
+  }
+  apply continued_simulation_rel in Hsim_ex'.
+  by apply Hsim_ex' in Htrace_end'.
+Qed.
 
-Lemma module_invariance {Σ} `{anerisPreG Σ unit_model} (N: namespace) ip
-  (Φ: ∀ `{anerisG Σ}, iProp Σ → val → iProp Σ)  (* Module specification *)
-  (P0: iProp Σ) (* Initial resources required by the module *)
-  (e: val → expr) (* Context program, parameterized by the module *)
-  (e_init: expr) (* Initialization code, used to allocate resources for P0 *)
-  (imimpl: val) (* Implementation of the module (instrumented) *)
-  (good_trace: list val → Prop) (* Trace property *)
-  (σ: state): (* Initial state *)
-  (* The initial trace must satisfy the property *)
+Lemma adequacy_trace {Σ} `{anerisPreG Σ unit_model} (N : namespace) ip
+  (Φ : ∀ `{anerisG Σ}, iProp Σ → val → iProp Σ)  (P0 : iProp Σ) 
+  (e : val → expr) (e_init : expr) (imimpl : val) (good_trace: list val → Prop) 
+  (σ: state) (A : gset socket_address) (IPs : gset ip_address) (lbls : gset string) 
+  (obs_send_sas : gset socket_address) (obs_rec_sas : gset socket_address) :
+  state_heaps σ = {[ip:=∅]} →
+  state_sockets σ = {[ip:=∅]} →
+  state_ms σ = ∅ →
+  state_trace σ = [] →
+  ip ∉ IPs →
+  obs_send_sas ⊆ A →
+  obs_rec_sas ⊆ A →
   good_trace (state_trace σ) →
-  (* The context must be safe, given a module satisfying the specification Φ *)
   (⊢ ∀ `(anerisG Σ) P m, Φ P m -∗ {{{ P }}} e m @[ip] {{{ v, RET v; True }}}) →
-  (* The initialization code must provide P0 *)
-  (⊢ ∀ `(anerisG Σ), {{{ True }}} e_init @[ip] {{{ v, RET v; P0 }}}) →
-  (* The implementation provided for the module (iops) must satisfy the specification Φ.
-     On top of P0 it is given SL resources for the trace. *)
+  (⊢ ∀ `(anerisG Σ), 
+    {{{ unallocated A ∗
+        ([∗ set] a ∈ A, a ⤳[bool_decide (a ∈ obs_send_sas), bool_decide (a ∈ obs_rec_sas)] (∅, ∅)) ∗
+        ([∗ set] ip ∈ IPs, free_ip ip) ∗
+        ([∗ set] lbl ∈ lbls, alloc_evs lbl []) ∗
+        ([∗ set] sa ∈ obs_send_sas, sendon_evs sa []) ∗
+        ([∗ set] sa ∈ obs_rec_sas, receiveon_evs sa []) ∗
+        observed_send obs_send_sas ∗
+        observed_receive obs_rec_sas }}} 
+    e_init @[ip] 
+    {{{ v, RET v; P0 }}}) →
   (⊢ ∀ `(anerisG Σ), Φ (P0 ∗ trace_is (state_trace σ) ∗ trace_inv N good_trace)%I imimpl) →
-  (* Then the trace remains good at every step *)
   ∀ σ' e',
-    step ([(mkExpr ip (e_init ;; e imimpl))], σ) (e', σ') →
+    rtc step ([(mkExpr ip (e_init ;; e imimpl))], σ) (e', σ') →
     good_trace (state_trace σ').
 Proof.
-  intros Htrσ Hctx Hinit Himpl σ' e' Hsteps.
-  eapply heap_invariance. done.
-  2: eapply Hsteps.
-  iIntros (?) "HI Htr". wp_bind e_init.
-  iApply Hinit; first done.
+  intros Hstate_heap Hstate_sock Hstate_ms Hstate_trace Hips_nin Hobs_send Hobs_rec.
+  intros Htr Hctx Hinit Himpl σ' e' Hsteps.
+  eapply (aneris_invariance _ _ _ _ _ A _ _ obs_send_sas obs_rec_sas); try done.
+  iIntros (? ?) "!# (#HI & Htr & Hunalloc & Hobs & Hfree_ip & Hlbs 
+    & Hsend_evs & Hrec_evs & Hobs_send & Hobs_rec) HΦ". 
+  wp_bind e_init. 
+  iApply (Hinit with "[$Hunalloc $Hobs $Hfree_ip $Hlbs $Hsend_evs $Hrec_evs 
+    $Hobs_send $Hobs_rec][Htr HΦ]").
   iNext.
-  iIntros (v) "H0". wp_pures.
-  iApply (Hctx with "[] [H0 Htr HI]").
+  iIntros (v) "H0". 
+  wp_pures.
+  iApply (Hctx with "[] [H0 Htr HI] [HΦ]").
   - iApply Himpl.
-  - iFrame.
-  - eauto.
+  - iFrame "∗#".
+  - done.
+Qed.
+
+Lemma adequacy_trace_simpl {Σ} `{anerisPreG Σ unit_model} (N : namespace) ip
+  (Φ : ∀ `{anerisG Σ}, iProp Σ → val → iProp Σ)  (P0 : iProp Σ) 
+  (e : val → expr) (e_init : expr) (imimpl : val) (good_trace: list val → Prop) 
+  (σ: state) (A : gset socket_address) (IPs : gset ip_address)  :
+  state_heaps σ = {[ip:=∅]} →
+  state_sockets σ = {[ip:=∅]} →
+  state_ms σ = ∅ →
+  state_trace σ = [] →
+  ip ∉ IPs →
+  good_trace (state_trace σ) →
+  (⊢ ∀ `(anerisG Σ) P m, Φ P m -∗ {{{ P }}} e m @[ip] {{{ v, RET v; True }}}) →
+  (⊢ ∀ `(anerisG Σ), 
+    {{{ unallocated A ∗ ([∗ set] a ∈ A, a ⤳ (∅, ∅)) ∗ ([∗ set] ip ∈ IPs, free_ip ip) }}} 
+    e_init @[ip] 
+    {{{ v, RET v; P0 }}}) →
+  (⊢ ∀ `(anerisG Σ), Φ (P0 ∗ trace_is (state_trace σ) ∗ trace_inv N good_trace)%I imimpl) →
+  ∀ σ' e',
+    rtc step ([(mkExpr ip (e_init ;; e imimpl))], σ) (e', σ') →
+    good_trace (state_trace σ').
+Proof.
+  intros Hstate_heap Hstate_sock Hstate_ms Hstate_trace Hips_nin.
+  intros Htr Hctx Hinit Himpl σ' e' Hsteps.
+  eapply (aneris_invariance _ _ _ _ _ A _ ∅ ∅ ∅); try done.
+  iIntros (? ?) "!# (#HI & Htr & Hunalloc & Hobs & Hfree_ip & Hlbs 
+    & Hsend_evs & Hrec_evs & Hobs_send & Hobs_rec) HΦ". 
+  wp_bind e_init. 
+  iApply (Hinit with "[$Hunalloc $Hfree_ip $Hobs][Htr HΦ]").
+  iNext.
+  iIntros (v) "H0". 
+  wp_pures.
+  iApply (Hctx with "[] [H0 Htr HI] [HΦ]").
+  - iApply Himpl.
+  - iFrame "∗#".
+  - done.
 Qed.
